update double example

theories/examples/double.v
@@ -3,99 +3,118 @@ From iris.base_logic.lib Require Import invariants.
 From iris.heap_lang Require Import notation proofmode lib.par lib.spin_lock.
 From iris.algebra Require Import agree frac csum excl frac_auth.
 From actris.channel Require Import proto_channel channel proofmode.
+From logrel_heaplang_sessions Require Export lty ltyping basic arr chan chan_proto.
 
-Definition prog (c : val) : expr :=
+Definition prog : val := λ: "c",
   let: "lock" := newlock #() in
-  (
+  let: "p" := (
     acquire "lock";;
-    recv c;;
-    release "lock"
+    let: "x1" := recv "c" in
+    release "lock";;
+    "x1"
   ) ||| (
     acquire "lock";;
-    recv c;;
-    release "lock"
-  );;
-  #().
+    let: "x2" := recv "c" in
+    release "lock";;
+    "x2"
+  ) in "p".
 
 Section GhostState.
-  Definition doubleR := frac_authR natR.
-  Class doubleG Σ := { double_inG :> inG Σ doubleR }.
-  Definition doubleΣ : gFunctors := #[GFunctor doubleR].
-  Instance subG_doubleΣ {Σ} : subG doubleΣ Σ → doubleG Σ.
-  Proof. solve_inG. Qed.
-
   Class fracG Σ := { frac_inG :> inG Σ fracR }.
   Definition fracΣ : gFunctors := #[GFunctor fracR].
   Instance subG_fracΣ {Σ} : subG fracΣ Σ → fracG Σ.
   Proof. solve_inG. Qed.
-
-  Definition auth (n : nat) : doubleR := ●F (n : natR).
-  Definition partial (q : Qp) (n : nat) : doubleR := ◯F{q} n.
 End GhostState.
 
 Section Double.
-  Context `{heapG Σ, proto_chanG Σ, doubleG Σ, fracG Σ}.
-
-  Lemma partial_split γ n:
-    own γ (partial 1 n) -∗ own γ (partial (1/2) n) ∗ own γ (partial (1/2) n).
-  Proof. Admitted.
-
-  Lemma partial_inc γ q n m:
-    own γ (auth n) ∗ own γ (partial q m) ==∗ own γ (auth (n + 1)) ∗ own γ (partial q (m + 1)).
-  Proof. Admitted.
+  Context `{heapG Σ, proto_chanG Σ, fracG Σ, spawnG Σ}.
 
   Definition proto_begin : iProto Σ :=
-    (<?> x1 : nat, MSG #x1; <?> x2 : nat, MSG #x2; END)%proto.
+    (<?> x1 : Z, MSG #x1; <?> x2 : Z, MSG #x2; END)%proto.
 
-  Definition chan_inv (c : val) (γ1 γ2 : gname) : iProp Σ :=
-    ((own γ1 (auth 0) ∗ c ↣ <?> x1 : nat, MSG #x1; <?> x2 : nat, MSG #x2; END) ∨
-     (own γ1 (auth 1) ∗ own γ2 (1/2)%Qp ∗ c ↣ <?> x2 : nat, MSG #x2; END) ∨
-     (own γ1 (auth 2) ∗ own γ2 1%Qp ∗ c ↣ END))%I.
+  Definition chan_inv (c : val) (γ : gname) : iProp Σ :=
+    ((c ↣ <?> x1 : Z, MSG #x1; <?> x2 : Z, MSG #x2; END) ∨
+     (own γ (1/2)%Qp ∗ c ↣ <?> x2 : Z, MSG #x2; END) ∨
+     (own γ 1%Qp ∗ c ↣ END))%I.
 
   Lemma wp_prog (N : namespace) (c : val):
-    {{{ c ↣ proto_begin }}} prog c {{{ v, RET v; ⌜v = #()⌝ }}}.
+    {{{ ▷ (c ↣ proto_begin) }}} prog c {{{ v, RET v; ∃ k1 k2 : Z, ⌜v = (#k1, #k2)%V⌝ }}}.
   Proof.
     iIntros (Φ) "Hc HΦ".
     rewrite /prog.
 
-    iMod (own_alloc (auth 0 ⋅ partial 1 0)) as (γ1) "[Hauth Hpartial]".
-    { admit. }
-    iMod (own_alloc 1%Qp) as (γ2) "[Hcredit1 Hcredit2]".
-    { admit. }
+    iMod (own_alloc 1%Qp) as (γ) "[Hcredit1 Hcredit2]".
+    { done. }
 
     (* Create lock *)
-    wp_apply (newlock_spec N (chan_inv c γ1 γ2) with "[Hc Hauth]").
-    { iLeft. iFrame "Hc Hauth". }
+    wp_apply (newlock_spec N (chan_inv c γ) with "[Hc]").
+    { iLeft. iFrame "Hc". }
     iIntros (lk γlk) "#Hlock".
     wp_pures.
 
-    iPoseProof (partial_split with "Hpartial") as "[Hpartial1 Hpartial2]".
-
     (* Fork into two threads *)
     wp_bind (par _ _).
-    wp_apply (wp_par (λ _, own γ1 (partial (1/2) 1)) (λ _, own γ1 (partial (1/2) 1)) with "[Hpartial1 Hcredit1]").
+    wp_apply (wp_par (λ v, ∃ k : Z, ⌜v = #k⌝)%I (λ v, ∃ k : Z, ⌜v = #k⌝)%I with "[Hcredit1] [Hcredit2]").
     - (* Acquire lock *)
       wp_apply (acquire_spec with "Hlock").
       iIntros "[Hlocked Hc]". wp_pures.
       iDestruct "Hc" as "[Hc|[Hc|Hc]]".
-      + iDestruct "Hc" as "[Hauth Hc]".
-        wp_recv (x1) as "_". wp_pures.
-        iMod (partial_inc with "[Hauth Hpartial1]") as "[Hauth Hpartial1]".
-        { iFrame "Hauth Hpartial1". }
-        wp_apply (release_spec with "[Hlocked Hcredit1 Hauth Hc]").
-        { iFrame "Hlock Hlocked". iRight. iLeft. iFrame "Hauth Hcredit1 Hc". }
+      + wp_recv (x1) as "_". wp_pures.
+        wp_apply (release_spec with "[Hlocked Hcredit1 Hc]").
+        { iFrame "Hlock Hlocked". iRight. iLeft. iFrame "Hcredit1 Hc". }
         iIntros "_". wp_pures.
-        iApply "Hpartial1".
-      +
-      + admit. (* Impossible due to fractions *)
-    - admit.
-  Admitted.
+        by iExists x1.
+      + iDestruct "Hc" as "[Hcredit2 Hc]".
+        wp_recv (x1) as "_". wp_pures.
+        iCombine "Hcredit1 Hcredit2" as "Hcredit".
+        wp_apply (release_spec with "[Hlocked Hcredit Hc]").
+        { iFrame "Hlock Hlocked". iRight. iRight. iFrame "Hcredit Hc". }
+        iIntros "_". wp_pures.
+        by iExists x1.
+      + iDestruct "Hc" as "[Hcredit2 Hc]".
+        iCombine "Hcredit1 Hcredit2" as "Hcredit".
+        iExFalso. iDestruct (own_valid with "Hcredit") as "%".
+        done.
+    - (* Acquire lock *)
+      wp_apply (acquire_spec with "Hlock").
+      iIntros "[Hlocked Hc]". wp_pures.
+      iDestruct "Hc" as "[Hc|[Hc|Hc]]".
+      + wp_recv (x1) as "_". wp_pures.
+        wp_apply (release_spec with "[Hlocked Hcredit2 Hc]").
+        { iFrame "Hlock Hlocked". iRight. iLeft. iFrame "Hcredit2 Hc". }
+        iIntros "_". wp_pures.
+        by iExists x1.
+      + iDestruct "Hc" as "[Hcredit1 Hc]".
+        wp_recv (x1) as "_". wp_pures.
+        iCombine "Hcredit1 Hcredit2" as "Hcredit".
+        wp_apply (release_spec with "[Hlocked Hcredit Hc]").
+        { iFrame "Hlock Hlocked". iRight. iRight. iFrame "Hcredit Hc". }
+        iIntros "_". wp_pures.
+        by iExists x1.
+      + iDestruct "Hc" as "[Hcredit1 Hc]".
+        iCombine "Hcredit1 Hcredit2" as "Hcredit".
+        iExFalso. iDestruct (own_valid with "Hcredit") as "%".
+        done.
+    - iIntros (x1 x2) "[Hx1 Hx2]".
+      iModIntro. wp_pures.
+      iApply "HΦ".
+      iDestruct "Hx1" as (k1) "->".
+      iDestruct "Hx2" as (k2) "->".
+      by iExists k1, k2.
+  Qed.
 
-  (* We need to prove using ghost state that at most two receives will
-  be performed in the beginning. Afterwards, we might be able to use
-  an agreement RA to have the two processes communicate the value they
-  have received and to determine who has the lowest one. Then the
-  invariant needs to ensure that only the process with the lowest
-  value can access it. *)
+  Lemma lty_prog (N : namespace):
+    ∅ ⊨ prog : chan (<??> lty_int; <??> lty_int; END) → (lty_int * lty_int).
+  Proof.
+    iIntros (vs) "_ /=".
+    wp_apply wp_value.
+    iModIntro. iIntros (c) "Hc".
+    wp_apply (wp_prog N with "[Hc]").
+    { iModIntro. admit. }
+    iIntros (r) "Hr".
+    iDestruct "Hr" as (k1 k2) "->".
+    iExists #k1, #k2. iSplit=> //.
+    iSplit; by eauto.
+  Admitted.
 
 End Double.
